common/AST.v
@@ -707,9 +707,6 @@ Proof.
     + rewrite !PTree.gso by auto. apply IHdefs.
 Qed.
 
-Lemma erase_program_is_internal p:
- 
-
 End ERASE_PROGRAM.
 
 (** * Arguments and results to builtin functions *)
